disk-betree/KMTable.i.dfy
@@ -1030,13 +1030,18 @@ module KMTable {
   lemma Ireplace1with2(kmts: seq<KMTable>, kmt1: KMTable, kmt2: KMTable, slot: int)
   requires WF(kmt1)
   requires WF(kmt2)
+  requires Bounded(kmt1)
+  requires Bounded(kmt2)
   requires 0 <= slot < |kmts|
   requires forall i | 0 <= i < |kmts| :: WF(kmts[i])
+  requires forall i | 0 <= i < |kmts| :: Bounded(kmts[i])
   ensures forall i | 0 <= i < |replace1with2(kmts, kmt1, kmt2, slot)| :: WF(replace1with2(kmts, kmt1, kmt2, slot)[i])
+  ensures forall i | 0 <= i < |replace1with2(kmts, kmt1, kmt2, slot)| :: Bounded(replace1with2(kmts, kmt1, kmt2, slot)[i])
   ensures ISeq(replace1with2(kmts, kmt1, kmt2, slot)) == replace1with2(ISeq(kmts), I(kmt1), I(kmt2), slot)
   {
     forall i | 0 <= i < |replace1with2(kmts, kmt1, kmt2, slot)|
     ensures WF(replace1with2(kmts, kmt1, kmt2, slot)[i])
+    ensures Bounded(replace1with2(kmts, kmt1, kmt2, slot)[i])
     {
       if i < slot {
         assert replace1with2(kmts, kmt1, kmt2, slot)[i] == kmts[i];
